A little Axpy

src/Appli/Fappli_Axpy.v
@@ -12,6 +12,64 @@ Variable Hp : Zlt 0 prec.
 
 Notation format := (generic_format beta (FLX_exp prec)).
 Notation cexp := (canonic_exponent beta (FLX_exp prec)).
+Notation ulp := (ulp beta (FLX_exp prec)).
+
+Definition MinOrMax x f := 
+   ((f = rounding beta (FLX_exp prec) ZrndDN x) 
+     \/ (f = rounding beta (FLX_exp prec) ZrndUP x)).
+
+Theorem MinOrMax_opp: forall x f,
+   MinOrMax x f <->  MinOrMax (-x) (-f).
+assert (forall x f, MinOrMax x f -> MinOrMax (- x) (- f)).
+unfold MinOrMax; intros x f [H|H].
+right.
+now rewrite H, rounding_UP_opp.
+left.
+now rewrite H, rounding_DN_opp.
+intros x f; split; intros H1.
+now apply H.
+rewrite <- (Ropp_involutive x), <- (Ropp_involutive f).
+now apply H.
+Qed.
+
+
+Theorem implies_MinOrMax_le:
+  forall x f, format f ->
+  (f <= x)%R ->
+  (Rabs (f-x) < ulp x)%R -> 
+  MinOrMax x f.
+intros x f Hf Hxf1 Hxf2.
+left; apply sym_eq.
+apply Rnd_DN_pt_unicity with format x.
+apply generic_DN_pt.
+now apply FLX_exp_correct.
+split;[assumption|idtac].
+split;[assumption|idtac].
+intros g Hg Hxg.
+case (Rle_or_lt g f); trivial; intros Hfg.
+contradict Hxf2.
+apply Rle_not_lt.
+rewrite Rabs_left1.
+2: apply Rle_minus; assumption.
+replace (-(f-x))%R with ((x-g)+(g-f))%R by ring.
+rewrite <- (Rplus_0_l (ulp x)).
+apply Rplus_le_compat.
+apply Rle_0_minus; assumption.
+Admitted.
+
+
+
+
+Theorem implies_MinOrMax_quarter:
+  forall x f, format f ->
+  (Rabs (f-x) < /4* ulp x)%R -> 
+  MinOrMax x f.
+intros x f Hf Hxf.
+Admitted.
+
+
+
+
 
 Variable choice : R -> bool.
 
@@ -23,9 +81,7 @@ Hypothesis Hy: format y.
 
 Notation t := (rounding beta (FLX_exp prec) (ZrndN choice) (a*x)).
 Notation u := (rounding beta (FLX_exp prec) (ZrndN choice) (t+y)).
-Notation MinOrMax x f := 
-   ((f = rounding beta (FLX_exp prec) ZrndUP x) 
-     \/ (f = rounding beta (FLX_exp prec) ZrndDN x)).
+
 
 
 Theorem Axpy_opt :
